update merge to be inductive so we don't need decidability. also changed cstep2 and estep2 to use regular impe exp and com. projection and merge now move from impe values to impe2 values. we need to prove stuff about non-nested pairs.

ImpE2.v
@@ -23,88 +23,11 @@ Require Import ImpE.
 *******************************************************************************)
 
 Section Syntax.
-  Inductive exp2 : Type :=
-  | Enat2 : nat -> exp2
-  | Evar2 : var -> exp2
-  | Eplus2 : exp2 -> exp2 -> exp2
-  | Emult2 : exp2 -> exp2 -> exp2
-  | Eloc2 : location -> exp2
-  | Ederef2 : exp2 -> exp2
-  | Eisunset2 : condition -> exp2
-  | Elambda2 : mode -> com2 -> exp2
-                                   
-  with com2 : Type :=
-  | Cskip2 : com2
-  | Cassign2 : var -> exp2 -> com2
-  | Cdeclassify2 : var -> exp2 -> com2
-  | Cupdate2 : exp2 -> exp2 -> com2
-  | Coutput2 : exp2 -> sec_level -> com2
-  | Ccall2 : exp2 -> com2
-  | Cset2 : condition -> com2
-  | Cenclave2 : enclave -> com2 -> com2
-  | Ckill2 : enclave -> com2
-  | Cseq2 : list com2 -> com2
-  | Cif2 : exp2 -> com2 -> com2 -> com2
-  | Cwhile2 : exp2 -> com2 -> com2.
-
   Inductive val2 : Type :=
-  | Vlambda2 : mode -> com2 -> val2
+  | Vlambda2 : mode -> com -> val2
   | Vnat2 : nat -> val2
   | Vloc2 : location -> val2
   | Vpair2 : val2 -> val2 -> val2.
-
-  Function forall_subexp2 (e: exp2) (P: exp2 -> Prop) : Prop :=
-    P e /\
-    match e with
-    | Eplus2 e1 e2 => forall_subexp2 e1 P /\ forall_subexp2 e2 P
-    | Emult2 e1 e2 => forall_subexp2 e1 P /\ forall_subexp2 e2 P
-    | Ederef2 e' => forall_subexp2 e' P
-    | Elambda2 _ c => forall_subexp2' c P
-    | _ => True
-    end
-  with forall_subexp2' (c: com2) (P: exp2 -> Prop) : Prop :=
-    match c with
-    | Cassign2 _ e => forall_subexp2 e P
-    | Cdeclassify2 _ e => forall_subexp2 e P
-    | Cupdate2 e1 e2 => forall_subexp2 e1 P /\ forall_subexp2 e2 P
-    | Ccall2 e => forall_subexp2 e P
-    | Cenclave2 _ c' => forall_subexp2' c' P
-    | Cseq2 cs => fold_left (fun acc c => forall_subexp2' c P /\ acc) cs True
-    | Cif2 e c1 c2 =>
-      forall_subexp2 e P /\ forall_subexp2' c1 P /\ forall_subexp2' c2 P
-    | Cwhile2 e c' => forall_subexp2 e P /\ forall_subexp2' c' P
-    | _ => True
-    end.
-
-   Ltac auto_decide :=
-    try match goal with
-    | [x : nat, y : nat |- _] => destruct (Nat.eq_dec x y)
-    | [x : var, y : var |- _] => destruct (Nat.eq_dec x y)
-    | [x : condition, y : condition |- _] => destruct (Nat.eq_dec x y)
-    | _ => idtac
-    end; [left; now subst | right; congruence].
-
-  Definition exp2_novars (e: exp2) : Prop :=
-    forall_subexp2 e (fun e =>
-                       match e with
-                       | Evar2 _ => False
-                       | _ => True
-                       end).
- 
-  Lemma com2_decidable : forall c1 c2 : com2, {c1 = c2} + {c1 <> c2}.
-  Admitted.
-
-  (* XXX I feel like it should be easy to prove this...? *)
-  Lemma val2_decidable : forall v1 v2 : val2, {v1 = v2} + {v1 <> v2}.
-  Proof.
-    intros.
-    destruct v1, v2; try (right; discriminate).
-    destruct (mode_decidable m m0); destruct (com2_decidable c c0); subst;
-    [left; auto | | | ]; right; congruence.
-    auto_decide.
-    destruct l, l0; try (right; discriminate); auto_decide.
-  Admitted.
-
 End Syntax.
 
 (*******************************************************************************
@@ -122,18 +45,18 @@ Section Semantics.
   | KPair: kill2 -> kill2 -> kill2.
 
   Inductive event2 : Type :=
-  | Emp : event2
-  | Decl : exp2 -> mem2 -> event2
-  | Mem : mem2 -> event2
-  | Out : sec_level -> val2 -> event2
-  | ANonEnc : com2 -> event2
-  (* XXX: need to add enc equiv definition for com2 *)
-  | AEnc : forall c c' : com2, (*enc_equiv c c'*) event2
-  | EPair : event2 -> event2 -> event2.
+  | Emp2 : event2
+  | Decl2 : exp -> mem2 -> event2
+  | Mem2 : mem2 -> event2
+  | Out2 : sec_level -> val2 -> event2
+  | ANonEnc2 : com -> event2
+  | AEnc2 : forall c c' : com, enc_equiv c c' -> event2
+  | EPair2 : event2 -> event2 -> event2.
   Definition trace2 : Type := list event2.
 
   (* Mode is only alive if it is alive in both of the kill sets in a pair *)
   (* XXX: not sure if this definition is right but it seems reasonable *)
+  (* Seems right---both sides of kill pair are equal when it's well-typed *)
   Function mode_alive2 (md : mode) (k : kill2) :=
     match md with
     | Normal => True
@@ -150,114 +73,145 @@ Section Semantics.
     | Normal => True
     | Encl _ => md = lmd /\ mode_alive2 lmd k
     end.
-  
-  Definition merge_reg (r1 r2: reg2) :=
-    fun x => if val2_decidable (r1 x) (r2 x) then r1 x
-             else Vpair2 (r1 x) (r2 x).
-  Definition merge_mem (m1 m2: mem2) :=
-    fun l => if val2_decidable (m1 l) (m2 l) then m1 l
-             else m2 l.
-  Definition tracepair_len (t: trace2 * trace2) := length (fst t) + length (snd t).
-  Function merge_trace (t: trace2 * trace2) {measure tracepair_len t} :=
+
+  Definition val_to_val2 (v: val) : val2 :=
+    match v with
+    | Vnat n => Vnat2 n
+    | Vlambda md c => Vlambda2 md c
+    | Vloc l => Vloc2 l
+    end.
+  Definition mem_to_mem2 (m: mem) : mem2 := fun x => val_to_val2 (m x).
+  Inductive merge_reg (r1 r2: reg) : reg2 -> Prop :=
+  | rmerge : forall r,
+      (forall x, r1 x <> r2 x -> r x = Vpair2 (val_to_val2 (r1 x)) (val_to_val2 (r2 x)))
+      -> (forall y, r1 y = r2 y -> r y = val_to_val2 (r1 y))
+      -> merge_reg r1 r2 r.
+  Inductive merge_mem (m1 m2: mem) : mem2 -> Prop :=
+  | mmerge : forall m,
+      (forall x, m1 x <> m2 x -> m x = Vpair2 (val_to_val2 (m1 x)) (val_to_val2 (m2 x)))
+      -> (forall y, m1 y = m2 y -> m y = val_to_val2 (m1 y))
+      -> merge_mem m1 m2 m.
+  Definition event_to_event2 (e: event) : event2 :=
+    match e with
+      | Mem m => Mem2 (mem_to_mem2 m)
+      | Decl e m => Decl2 e (mem_to_mem2 m)
+      | Out l v => Out2 l (val_to_val2 v)
+      | ANonEnc c => ANonEnc2 c
+      | AEnc c1 c2 enc_equiv => AEnc2 c1 c2 enc_equiv
+      | Emp => Emp2
+    end.
+  Definition tracepair_len (t: trace * trace) := length (fst t) + length (snd t).
+  Function merge_trace (t: trace * trace) {measure tracepair_len t} : trace2 :=
     match fst t, snd t with
-    | a1::tl1, a2::tl2 => EPair a1 a2 :: (merge_trace (tl1, tl2))
-    | a1::tl1, [] => EPair a1 Emp :: merge_trace (tl1, [])
-    | [], a2::tl2 => EPair Emp a2 :: merge_trace ([], tl2)
+    | a1::tl1, a2::tl2 => EPair2 (event_to_event2 a1)
+                                 (event_to_event2 a2) :: (merge_trace (tl1, tl2))
+    | a1::tl1, [] => EPair2 (event_to_event2 a1) Emp2 :: merge_trace (tl1, [])
+    | [], a2::tl2 => EPair2 Emp2 (event_to_event2 a2) :: merge_trace ([], tl2)
     | _, _ => []
     end.
   Proof. all: intros; unfold tracepair_len; rewrite teq, teq0; simpl; omega. Qed.
-  Definition merge_kill (k1 k2: kill2) := KPair k1 k2.
+  Definition merge_kill (k1 k2: set enclave) := KPair (KSingle k1) (KSingle k2).
   
-  Definition project_value (v : val2) (is_left : bool) : val2 :=
+  Function project_value (v: val2) (is_left: bool): val :=
     match v with
-    | Vpair2 v1 v2 => if is_left then v1 else v2
-    | _ => v
+      (* XXX pretty sure we can't have nested value pairs *)
+    | Vpair2 v1 v2 => if is_left then (project_value v1 is_left) else (project_value v2 is_left)
+    | Vnat2 v => Vnat v 
+    | Vlambda2 md c => Vlambda md c
+    | Vloc2 v => Vloc v
     end.
-  
-  Definition project_reg (r: reg2) (is_left : bool): reg2 :=
+  Definition project_reg (r: reg2) (is_left : bool): reg :=
     fun x => match r x with
-             | Vpair2 v1 v2 => if is_left then v1 else v2
-             | _ => r x
+             | Vpair2 v1 v2 => if is_left then project_value v1 is_left
+                               else project_value v2 is_left
+             | _ => project_value (r x) is_left
           end.
-
-  Definition project_mem (m: mem2) (is_left : bool): mem2 :=
+  Definition project_mem (m: mem2) (is_left : bool): mem :=
     fun x => match m x with
-          | Vpair2 v1 v2 => if is_left then v1 else v2
-          | _ => m x
+             | Vpair2 v1 v2 => if is_left then project_value v1 is_left
+                               else project_value v2 is_left
+             | _ => project_value (m x) is_left
           end.
-
-  Definition project_kill (k: kill2) (is_left : bool) : kill2 :=
+  (* XXX again need to show that kill pairs are never nested *)
+  Function project_kill (k: kill2) (is_left : bool) : set enclave :=
     match k with
-    | KPair ks1 ks2 => if is_left then ks1 else ks2
-    | _ => k
+    | KPair ks1 ks2 => if is_left then project_kill ks1 is_left
+                       else project_kill ks2 is_left
+    | KSingle k => k
     end.
-
-  Function project_trace (t: trace2) (is_left : bool) : trace2 :=
+  (* XXX show event pairs are never nested *)
+  Function event2_to_event (e: event2) (is_left: bool): event :=
+     match e with
+      | Mem2 m => Mem (project_mem m is_left)
+      | Decl2 e m => Decl e (project_mem m is_left)
+      | Out2 l v => Out l (project_value v is_left)
+      | ANonEnc2 c => ANonEnc c
+      | AEnc2 c1 c2 enc_equiv => AEnc c1 c2 enc_equiv
+      | EPair2 e1 e2 => if is_left then event2_to_event e1 is_left
+                        else event2_to_event e2 is_left
+      | Emp2 => Emp
+     end.
+  Function project_trace (t: trace2) (is_left : bool) : trace :=
     match t with
     | [] => []
-    | hd :: tl =>
-      let tl_proj := (project_trace tl is_left) in
-      match hd with
-      | Mem m => Mem (project_mem m is_left) :: tl_proj
-      | Decl e m => Decl e (project_mem m is_left) :: tl_proj
-      | Out l v => Out l (project_value v is_left) :: tl_proj
-      | ANonEnc _ | AEnc _ _ => hd :: tl_proj
-      | EPair e1 e2 => if is_left then e1 :: tl_proj else e2 :: tl_proj
-      | _ => []
+    | hd :: tl => let hd_proj := (event2_to_event hd is_left) in
+      match hd_proj with
+      | Emp => project_trace tl is_left
+      | _ => hd_proj :: project_trace tl is_left
       end
     end.
   
-  Definition econfig2 : Type := exp2 * reg2 * mem2 * kill2.
-  Definition ecfg_exp2 (ecfg: econfig2) : exp2 :=
+  Definition econfig2 : Type := exp * reg2 * mem2 * kill2.
+  Definition ecfg_exp2 (ecfg: econfig2) : exp :=
     match ecfg with (e, _, _, _) => e end.
   Definition ecfg_reg2 (ecfg: econfig2) : reg2 :=
     match ecfg with (_, r, _, _) => r end.
   Definition ecfg_mem2 (ecfg: econfig2) : mem2 :=
     match ecfg with (_, _, m, _) => m end.
-  Definition ecfg_update_exp2 (ecfg: econfig2) (e: exp2) : econfig2 :=
+  Definition ecfg_update_exp2 (ecfg: econfig2) (e: exp) : econfig2 :=
     match ecfg with (_, r, m, k) => (e, r, m, k) end.
   Definition esemantics2 : Type := mode -> loc_mode -> econfig2 -> val2 -> Prop.
 
   Inductive estep2 : esemantics2 :=
   | Estep2_nat : forall md d ecfg n,
-      ecfg_exp2 ecfg = Enat2 n ->
+      ecfg_exp2 ecfg = Enat n ->
       estep2 md d ecfg (Vnat2 n)
   | Estep2_loc : forall md d ecfg l,
-      ecfg_exp2 ecfg = Eloc2 l ->
+      ecfg_exp2 ecfg = Eloc l ->
       estep2 md d ecfg (Vloc2 l)
   | Estep2_lambda : forall md d ecfg c,
-      ecfg_exp2 ecfg = Elambda2 md c ->
+      ecfg_exp2 ecfg = Elambda md c ->
       estep2 md d ecfg (Vlambda2 md c)
   | Estep2_var : forall md d ecfg x v,
-      ecfg_exp2 ecfg = Evar2 x ->
+      ecfg_exp2 ecfg = Evar x ->
       ecfg_reg2 ecfg x = v ->
       estep2 md d ecfg v
   | Estep2_plus : forall md d ecfg e1 e2 n1 n2,
-      ecfg_exp2 ecfg = Eplus2 e1 e2 ->
+      ecfg_exp2 ecfg = Eplus e1 e2 ->
       estep2 md d (ecfg_update_exp2 ecfg e1) (Vnat2 n1) ->
       estep2 md d (ecfg_update_exp2 ecfg e2) (Vnat2 n2) ->
       estep2 md d ecfg (Vnat2 (n1 + n2))
   | Estep2_mult : forall md d ecfg e1 e2 n1 n2,
-      ecfg_exp2 ecfg = Emult2 e1 e2 ->
+      ecfg_exp2 ecfg = Emult e1 e2 ->
       estep2 md d (ecfg_update_exp2 ecfg e1) (Vnat2 n1) ->
       estep2 md d (ecfg_update_exp2 ecfg e2) (Vnat2 n2) ->
       estep2 md d ecfg (Vnat2 (n1 * n2))
   | Estep2_deref : forall md d ecfg e r m k l v,
-      ecfg = (Ederef2 e, r, m, k) ->
+      ecfg = (Ederef e, r, m, k) ->
       estep2 md d (e, r, m, k) (Vloc2 l) ->
       m l = v ->
       mode_access_ok2 md d l k ->
       estep2 md d ecfg v
   | Estep2_isunset : forall md d ecfg cnd v res,
-      ecfg_exp2 ecfg = Eisunset2 cnd ->
-      estep2 md d (ecfg_update_exp2 ecfg (Ederef2 (Eloc2 (Cnd cnd)))) v ->
+      ecfg_exp2 ecfg = Eisunset cnd ->
+      estep2 md d (ecfg_update_exp2 ecfg (Ederef (Eloc (Cnd cnd)))) v ->
       (v = Vnat2 0 /\ res = Vnat2 1) \/ (v <> Vnat2 0 /\ res = Vnat2 0) ->
       estep2 md d ecfg res.
 
   (* Semantics for commands. *)
-  Definition cconfig2 : Type := com2 * reg2 * mem2 * kill2.
+  Definition cconfig2 : Type := com * reg2 * mem2 * kill2.
   Definition cterm2 : Type := reg2 * mem2 * kill2.
-  Definition ccfg_com2 (ccfg: cconfig2) : com2 :=
+  Definition ccfg_com2 (ccfg: cconfig2) : com :=
     match ccfg with (c, _, _, _) => c end.
   Definition ccfg_reg2 (ccfg: cconfig2) : reg2 :=
     match ccfg with (_, r, _, _) => r end.
@@ -271,9 +225,9 @@ Section Semantics.
   Definition ccfg_update_reg2 (ccfg: cconfig2) (x: var) (v: val2) : reg2 :=
     fun var => if var =? x then v
                else (ccfg_reg2 ccfg) var.
-  Definition ccfg_to_ecfg2 (e: exp2) (ccfg : cconfig2) : econfig2 :=
+  Definition ccfg_to_ecfg2 (e: exp) (ccfg : cconfig2) : econfig2 :=
     (e, (ccfg_reg2 ccfg), (ccfg_mem2 ccfg), (ccfg_kill2 ccfg)).
-  Definition ccfg_update_com2 (c: com2) (ccfg : cconfig2) : cconfig2 :=
+  Definition ccfg_update_com2 (c: com) (ccfg : cconfig2) : cconfig2 :=
     (c, (ccfg_reg2 ccfg), (ccfg_mem2 ccfg), (ccfg_kill2 ccfg)).
   Definition csemantics2 : Type := mode -> loc_mode -> cconfig2 -> cterm2 -> trace2 -> Prop.  
 
@@ -281,20 +235,20 @@ Section Semantics.
   | Cstep2_skip : forall md d ccfg,
       cstep2 md d ccfg (ccfg_reg2 ccfg, ccfg_mem2 ccfg, ccfg_kill2 ccfg) []
   | Cstep2_assign : forall md d ccfg x e v r',
-      ccfg_com2 ccfg = Cassign2 x e ->
+      ccfg_com2 ccfg = Cassign x e ->
       estep2 md d (ccfg_to_ecfg2 e ccfg) v ->
       r' = ccfg_update_reg2 ccfg x v ->
       mode_alive2 md (ccfg_kill2 ccfg) ->
       cstep2 md d ccfg (r', ccfg_mem2 ccfg, ccfg_kill2 ccfg) []
   | Cstep2_declassify : forall md d ccfg x e v r',
-      ccfg_com2 ccfg = Cdeclassify2 x e ->
-      exp2_novars e ->
+      ccfg_com2 ccfg = Cdeclassify x e ->
+      exp_novars e ->
       estep2 md d (ccfg_to_ecfg2 e ccfg) v ->
       r' = ccfg_update_reg2 ccfg x v ->
       mode_alive2 md (ccfg_kill2 ccfg) ->
-      cstep2 md d ccfg (r', ccfg_mem2 ccfg, ccfg_kill2 ccfg) [Decl e (ccfg_mem2 ccfg)]
+      cstep2 md d ccfg (r', ccfg_mem2 ccfg, ccfg_kill2 ccfg) [Decl2 e (ccfg_mem2 ccfg)]
   | Cstep2_update : forall md d ccfg e1 e2 l v m',
-      ccfg_com2 ccfg = Cupdate2 e1 e2 ->
+      ccfg_com2 ccfg = Cupdate e1 e2 ->
       estep2 md d (ccfg_to_ecfg2 e1 ccfg) (Vloc2 l) ->
       estep2 md d (ccfg_to_ecfg2 e2 ccfg) v ->
       mode_alive2 md (ccfg_kill2 ccfg) ->
@@ -303,72 +257,77 @@ Section Semantics.
       m' = ccfg_update_mem2 ccfg l v ->
       cstep2 md d ccfg (ccfg_reg2 ccfg, m', ccfg_kill2 ccfg) []
   | Cstep2_output : forall md d ccfg e sl v,
-      ccfg_com2 ccfg = Coutput2 e sl ->
+      ccfg_com2 ccfg = Coutput e sl ->
       estep2 md d (ccfg_to_ecfg2 e ccfg) v ->
       sl = L \/ sl = H ->
       mode_alive2 md (ccfg_kill2 ccfg) ->
       cstep2 md d ccfg (ccfg_reg2 ccfg, ccfg_mem2 ccfg, ccfg_kill2 ccfg)
-            [Mem (ccfg_mem2 ccfg); Out sl v]
+            [Mem2 (ccfg_mem2 ccfg); Out2 sl v]
   | Cstep2_call : forall md d ccfg e c r' m' k' tr,
-      ccfg_com2 ccfg = Ccall2 e ->
+      ccfg_com2 ccfg = Ccall e ->
       estep2 md d (ccfg_to_ecfg2 e ccfg) (Vlambda2 md c) ->
       cstep2 md d (ccfg_update_com2 c ccfg) (r', m', k') tr ->
       cstep2 md d ccfg (r', m', k') tr
   | Cstep2_cset : forall md d ccfg c m',
-      ccfg_com2 ccfg = Cset2 c ->
+      ccfg_com2 ccfg = Cset c ->
       mode_access_ok2 md d (Cnd c) (ccfg_kill2 ccfg) ->
       m' = ccfg_update_mem2 ccfg (Cnd c) (Vnat2 1) ->
-      mode_alive2 md (ccfg_kill2 ccfg) ->      cstep2 md d ccfg (ccfg_reg2 ccfg, m', ccfg_kill2 ccfg) [Mem m']
+      mode_alive2 md (ccfg_kill2 ccfg) ->
+      cstep2 md d ccfg (ccfg_reg2 ccfg, m', ccfg_kill2 ccfg) [Mem2 m']
   | Cstep2_enclave : forall md d ccfg enc c r' m' k' tr,
     md = Normal ->
-    ccfg_com2 ccfg = Cenclave2 enc c ->
+    ccfg_com2 ccfg = Cenclave enc c ->
     cstep2 (Encl enc) d (c, ccfg_reg2 ccfg, ccfg_mem2 ccfg, ccfg_kill2 ccfg) (r', m', k') tr ->
     cstep2 md d ccfg (r', m', k') tr
   | Cstep2_seq_nil : forall md d ccfg,
-      ccfg_com2 ccfg = Cseq2 [] ->
+      ccfg_com2 ccfg = Cseq [] ->
       cstep2 md d ccfg (ccfg_reg2 ccfg, ccfg_mem2 ccfg, ccfg_kill2 ccfg) []
   | Cstep2_seq_hd : forall md d ccfg hd tl r m k tr r' m' k' tr',
-      ccfg_com2 ccfg = Cseq2 (hd::tl) ->
+      ccfg_com2 ccfg = Cseq (hd::tl) ->
       cstep2 md d (ccfg_update_com2 hd ccfg) (r, m, k) tr ->
-      cstep2 md d (Cseq2 tl, r, m, k) (r', m', k') tr' ->
+      cstep2 md d (Cseq tl, r, m, k) (r', m', k') tr' ->
       cstep2 md d ccfg (r', m', k') (tr++tr')
   | Cstep2_if : forall md d ccfg e c1 c2 n r' m' k' tr,
-      ccfg_com2 ccfg = Cif2 e c1 c2 ->
+      ccfg_com2 ccfg = Cif e c1 c2 ->
       estep2 md d (ccfg_to_ecfg2 e ccfg) (Vnat2 n) ->
       ~(n = 0) ->
       cstep2 md d (ccfg_update_com2 c1 ccfg) (r', m', k') tr ->
       cstep2 md d ccfg (r', m', k') tr
   | Cstep2_else : forall md d ccfg e c1 c2 n r' m' k' tr,
-      ccfg_com2 ccfg = Cif2 e c1 c2 ->
+      ccfg_com2 ccfg = Cif e c1 c2 ->
       estep2 md d (ccfg_to_ecfg2 e ccfg) (Vnat2 n) ->
       (n = 0) ->
       cstep2 md d (ccfg_update_com2 c2 ccfg) (r', m', k') tr ->
       cstep2 md d ccfg (r', m', k') tr
-  | Cstep2_if_div : forall md d ccfg e c1 c2 n1 n2 r1 m1 k1 t1 r2 m2 k2 t2,
-      ccfg_com2 ccfg = Cif2 e c1 c2 ->
+  | Cstep2_if_div : forall md d ccfg e c1 c2 n1 n2 r1 m1 k1 t1 r2 m2 k2 t2 rmerge mmerge,
+      ccfg_com2 ccfg = Cif e c1 c2 ->
       estep2 md d (ccfg_to_ecfg2 e ccfg) (Vpair2 (Vnat2 n1) (Vnat2 n2)) ->
       let cleft := (match n1 with
                     | 0 => c2
                     | _ => c1 end) in
-      cstep2 md d (cleft, project_reg (ccfg_reg2 ccfg) true,
-                   project_mem (ccfg_mem2 ccfg) true, project_kill (ccfg_kill2 ccfg) true)
+      cstep md d (cleft, project_reg (ccfg_reg2 ccfg) true,
+                  project_mem (ccfg_mem2 ccfg) true,
+                  project_kill (ccfg_kill2 ccfg) true)
              (r1, m1, k1) t1 ->
       let cright := (match n2 with
                      | 0 => c2
                      | _ => c1 end) in
-      cstep2 md d (cright, project_reg (ccfg_reg2 ccfg) false,
-                   project_mem (ccfg_mem2 ccfg) false, project_kill (ccfg_kill2 ccfg) false)
-             (r2, m2, k2) t2 ->
-      cstep2 md d ccfg (merge_reg r1 r2, merge_mem m1 m2, merge_kill k1 k2) (merge_trace (t1, t2))
+      cstep md d (cright, project_reg (ccfg_reg2 ccfg) false,
+                  project_mem (ccfg_mem2 ccfg) false,
+                  project_kill (ccfg_kill2 ccfg) false)
+            (r2, m2, k2) t2 ->
+      merge_reg r1 r2 rmerge ->
+      merge_mem m1 m2 mmerge ->
+      cstep2 md d ccfg (rmerge, mmerge, merge_kill k1 k2) (merge_trace (t1, t2))
   | Cstep_while_t : forall md d ccfg e c v r m k tr r' m' k' tr',
-      ccfg_com2 ccfg = Cwhile2 e c ->
+      ccfg_com2 ccfg = Cwhile e c ->
       estep2 md d (ccfg_to_ecfg2 e ccfg) v ->
       ~(v = (Vnat2 0)) ->
       cstep2 md d (ccfg_update_com2 c ccfg) (r, m, k) tr ->
-      cstep2 md d (ccfg_update_com2 (Cwhile2 e c) ccfg) (r', m', k') tr' ->
+      cstep2 md d (ccfg_update_com2 (Cwhile e c) ccfg) (r', m', k') tr' ->
       cstep2 md d ccfg (r', m', k') (tr++tr')
   | Cstep_while_f : forall md d ccfg e c,
-      ccfg_com2 ccfg = Cwhile2 e c ->
+      ccfg_com2 ccfg = Cwhile e c ->
       estep2 md d (ccfg_to_ecfg2 e ccfg) (Vnat2 0) ->
       mode_alive2 md (ccfg_kill2 ccfg) ->
       cstep2 md d ccfg (ccfg_reg2 ccfg, ccfg_mem2 ccfg, ccfg_kill2 ccfg) []
@@ -376,7 +335,7 @@ Section Semantics.
   (* XXX: add in set add for pairs
   | Cstep_kill : forall md d ccfg enc,
       md = Normal ->
-      ccfg_com2 ccfg = Ckill2 enc ->
+      ccfg_com2 ccfg = Ckill enc ->
       mode_alive2 (Encl enc) (ccfg_kill2 ccfg) ->
       cstep2 md d ccfg (ccfg_reg2 ccfg, ccfg_mem2 ccfg, set_add Nat.eq_dec enc (ccfg_kill2 ccfg)) []*).
 End Semantics.
@@ -725,16 +684,19 @@ Section Adequacy.
   Proof.
   Admitted.
 
-  
-  
-    
   (* XXX this theorem statement doesn't work because the projection functions return back
      the xxx2 types for ImpE2 where we need the types for IMPE... *)
-Lemma impe2_sound : forall md d c r m K r' m' K' t,
+  
+  Lemma impe2_sound : forall md d c r m K r' m' K' t,
     cstep2 md d (c, r, m, K) (r', m', K') t ->
     (cstep md d (c, project_reg r true, project_mem m true, project_kill K true)
-           (project_reg r' true, project_mem m' true, project_kill K' true) project_trace t true) /\
+           (project_reg r' true, project_mem m' true, project_kill K' true)
+           (project_trace t true)) /\
     (cstep md d (c, project_reg r false, project_mem m false, project_kill K false)
-           (project_reg r' false, project_mem m' true, project_kill K' false) project_trace t false) *)
+           (project_reg r' false, project_mem m' true, project_kill K' false)
+           (project_trace t false)).
+  Proof.
+  Admitted.
+  
   
 End Adequacy.
